aneris/examples/reliable_communication/lib/repdb/proof/follower/proof_of_proxy.v
@@ -1,0 +1,120 @@
+From iris.algebra.lib Require Import mono_list.
+From iris.base_logic Require Import invariants.
+From iris.bi.lib Require Import fractional.
+From iris.proofmode Require Import tactics coq_tactics reduction spec_patterns.
+From aneris.lib Require Import gen_heap_light.
+From aneris.aneris_lang Require Import lang resources inject tactics proofmode.
+From aneris.aneris_lang.lib Require Import list_proof monitor_proof lock_proof map_proof.
+From aneris.aneris_lang.lib.serialization Require Import serialization_proof.
+From aneris.aneris_lang.program_logic Require Import aneris_lifting.
+From aneris.aneris_lang.program_logic Require Import aneris_weakestpre.
+From aneris.examples.reliable_communication.prelude
+     Require Import ser_inj.
+From aneris.examples.reliable_communication.lib.mt_server
+     Require Import user_params mt_server_code.
+From aneris.examples.reliable_communication.lib.mt_server.spec
+     Require Import api_spec.
+From aneris.examples.reliable_communication.lib.repdb
+     Require Import repdb_code model.
+From aneris.examples.reliable_communication.lib.repdb.spec
+     Require Import db_params time events.
+From aneris.examples.reliable_communication.lib.repdb.resources
+     Require Import
+     ras
+     resources_def
+     resources_global_inv
+     resources_local_inv.
+From aneris.examples.reliable_communication.lib.repdb.proof
+     Require Import
+     repdb_serialization.
+From aneris.examples.reliable_communication.lib.repdb.proof.follower
+     Require Import
+     clients_at_follower_mt_user_params
+     proof_of_clients_handler.
+
+Section Client_Proxy_Proof.
+  Context `{!anerisG Mdl Σ, dbparams : !DB_params, !IDBG Σ}.
+  Context (γL γM γF : gname).
+  Context (fsa : socket_address).
+  Context (Hin : fsa ∈ DB_followers).
+  Context (follower_si : message → iProp Σ).
+  Notation MTC := (client_handler_at_follower_user_params γL γM γF fsa).
+  Context (HClient_proxySpec :
+          ⊢ (∀ A sa, @init_client_proxy_spec _ _ _ _ MTC follower_si A sa)).
+
+  Definition read_at_follower_spec_internal
+           (rd : val) (csa fsaddr : socket_address) (k : Key) (h : wrlog) : iProp Σ :=
+      ⌜k ∈ DB_keys⌝ -∗
+    {{{ known_replog_token fsa γF ∗ own_logL_obs γL h ∗ own γF (◯ML h) }}}
+      rd #k @[ip_of_address csa]
+    {{{vo, RET vo;
+          ∃ h', ⌜h ≤ₚ h'⌝ ∗ own_obs γL fsaddr h' ∗
+         ((⌜vo = NONEV⌝ ∗ ⌜at_key k h' = None⌝) ∨
+         (∃ a, ⌜vo = SOMEV (we_val a)⌝ ∗ ⌜at_key k h' = Some a⌝))
+    }}}%I.
+
+ (* Definition read_at_follower_spec_internal *)
+ (*           (rd : val) (csa fsaddr : socket_address) (k : Key) (h : wrlog) : iProp Σ := *)
+ (*      ⌜k ∈ DB_keys⌝ -∗ *)
+ (*    {{{ own_obs γL fsaddr h }}} *)
+ (*      rd #k @[ip_of_address csa] *)
+ (*    {{{vo, RET vo; *)
+ (*          ∃ h', ⌜h ≤ₚ h'⌝ ∗ own_obs γL fsaddr h' ∗ *)
+ (*         ((⌜vo = NONEV⌝ ∗ ⌜at_key k h' = None⌝) ∨ *)
+ (*         (∃ a, ⌜vo = SOMEV (we_val a)⌝ ∗ ⌜at_key k h' = Some a⌝)) *)
+ (*    }}}%I. *)
+
+   Definition init_client_proxy_follower_spec_internal A csa : iProp Σ :=
+     ⌜fsa ≠ DB_addr⌝ →
+     ⌜fsa ∈ A⌝ →
+     ⌜csa ∉ A⌝ →
+     {{{ fixed A ∗
+         fsa ⤇ follower_si ∗
+         csa ⤳ (∅, ∅) ∗
+         free_ports (ip_of_address csa) {[port_of_address csa]} }}}
+       init_client_follower_proxy (s_serializer DB_serialization)
+         #csa #fsa @[ip_of_address csa]
+     {{{ rd, RET rd;
+         (∀ k h, read_at_follower_spec_internal rd csa fsa k h) }}}.
+
+  Lemma init_client_proxy_follower_internal_holds A sa :
+    Global_Inv γL γM ⊢ init_client_proxy_follower_spec_internal A sa.
+  Proof.
+    iIntros "#Hinv".
+    iIntros (Hneq HA HnA).
+    iIntros (Φ) "!#".
+    iIntros "(#Hf & #Hsi & Hmh & Hfp) HΦ".
+    rewrite /init_client_follower_proxy.
+    wp_pures.
+    wp_apply (HClient_proxySpec with "[$Hf $Hfp $Hmh $Hsi][HΦ]"); first done.
+    iNext.
+    iIntros (reqh) "#Hspec".
+    iApply "HΦ".
+    iIntros (k h).
+    rewrite /read_at_follower_spec_internal.
+    iIntros (Hkeys Ψ) "!#".
+    iIntros "Hobs HΨ".
+    wp_apply ("Hspec" $! _ (k, h) with "[Hobs]").
+    - iSplit.
+      -- iPureIntro. apply _.
+      -- iDestruct "Hobs" as "(#Hknw & #HobsL & #HobsF)".
+         iFrame "#".
+         iExists k, h.
+         by iFrame "#∗".
+    - iIntros (repd repv) "Hpost".
+      iApply "HΨ".
+      simplify_eq /=.
+      rewrite /ReqPost.
+      iDestruct "Hpost"
+        as (k' h0 h1) "(%Heq1 & -> & %Hpre & #Hknw & #HobsL1 & #HobsF1 & #Hpost)".
+      iExists h1.
+      inversion Heq1; subst.
+      iSplit; first done.
+      iSplit.
+      { iFrame "#". iRight. rewrite /own_replog_obs. iExists γF. iFrame "#". }
+      iDestruct "Hpost" as "[%Hpost|Hpost]".
+      -- iLeft. naive_solver.
+      -- iRight. naive_solver.
+  Qed.
+
+End Client_Proxy_Proof.
