aneris/examples/reliable_communication/lib/repdb/spec/ras.v
@@ -10,10 +10,10 @@ Class DBG `{!DB_time} Σ :=
   { DBG_Global_mem :> inG Σ (authR (gen_heapUR Key (option we)));
     DBG_Global_history_mono :> inG Σ (mono_listUR (leibnizO we));
     DBG_Known_replog :> inG Σ (authR (gmapUR socket_address (agreeR gnameO)));
-    DBG_free_replogG :> inG Σ (gset_disjUR socket_address);
+    (* DBG_free_replogG :> inG Σ (gset_disjUR socket_address); *)
     DBG_lockG :> lockG Σ;
     DBG_known_replog_name : gname;
-    DBG_free_replog_set_name : gname;
+    (* DBG_free_replog_set_name : gname; *)
   }.
 
 Class DBPreG `{!DB_time} Σ :=
@@ -21,7 +21,7 @@ Class DBPreG `{!DB_time} Σ :=
     DB_preG_Global_history_mono :> inG Σ (mono_listUR (leibnizO we));
     DB_preG_Known_replog :>
       inG Σ (authR (gmapUR socket_address (agreeR gnameO)));
-    DB_preG_free_replogG :> inG Σ (gset_disjUR socket_address);
+    (* DB_preG_free_replogG :> inG Σ (gset_disjUR socket_address); *)
     DB_preG_lockG :> lockG Σ;
   }.
 
@@ -29,7 +29,7 @@ Definition DBΣ `{!DB_time} : gFunctors :=
   #[GFunctor (authR (gen_heapUR Key (option we)));
     GFunctor (mono_listUR (leibnizO we));
     GFunctor (authR (gmapUR socket_address (agreeR gnameO)));
-    GFunctor (gset_disjUR socket_address);
+    (* GFunctor (gset_disjUR socket_address); *)
     lockΣ].
 
 Instance subG_DB_preGΣ `{!DB_time, !lockG Σ} : subG DBΣ Σ → DBPreG Σ.
